ulib/FStar.Heap.fst
@@ -17,7 +17,7 @@ abstract type heap = h:heap_rec{(forall (n:nat). n >= h.next_addr ==> None? (h.m
 private let consistent (h0:heap) (h1:heap)
   = forall n x y. (h0.memory n == Some x /\ h1.memory n == Some y) ==> dfst x == dfst y
 
-(* References: address * initial value *)
+(* References: address * initial value * manually managed flag *)
 abstract noeq type ref (a:Type0) = {
   addr: nat;
   init: a;
@@ -34,6 +34,14 @@ abstract let compare_addrs (#a:Type) (#b:Type) (r1:ref a) (r2:ref b)
 
 abstract let contains (#a:Type0) (h:heap) (r:ref a)
   = Some? (h.memory r.addr) /\ dfst (Some?.v (h.memory r.addr)) == a
+
+abstract let unused_in (#a:Type) (r:ref a) (h:heap) :Type0
+  = None? (h.memory r.addr)
+
+let fresh (#a:Type) (r:ref a) (h0:heap) (h1:heap) =
+  r `unused_in` h0 /\ h1 `contains` r
+
+let only x = singleton (addr_of x)
 
 (* Select. *)
 private abstract let sel_tot (#a:Type) (h:heap) (r:ref a{h `contains` r}) :a
@@ -67,162 +75,143 @@ abstract let upd (#a:Type) (h:heap) (r:ref a) (x:a) :GTot heap
                                   else h.memory r') }
 
 (* Allocate. *)
-abstract let alloc (#a:Type) (h:heap) (x:a) :GTot (ref a * heap)
-  = let r = { addr = h.next_addr; init = x; mm = false } in
+abstract let alloc (#a:Type) (h:heap) (x:a) (mm:bool) :GTot (ref a * heap)
+  = let r = { addr = h.next_addr; init = x; mm = mm } in
     r, upd #a h r x
 
-abstract let alloc_mm (#a:Type) (h:heap) (x:a)
-  :Ghost (ref a * heap) (requires True) (ensures (fun (r, _) -> is_mm r))
-  = let r = { addr = h.next_addr; init = x; mm = true } in
-    r, upd #a h r x
-
-private let contains_not_necessarily_well_typed (#a:Type) (h:heap) (r:ref a) :Type0 = Some? (h.memory r.addr)
-
-abstract let does_not_contain (#a:Type) (h:heap) (r:ref a) :Type0 = ~ (contains_not_necessarily_well_typed h r)
-
-(*
- * AR: the precondition here is stronger, we only require h `contains_not_necessarily_well_typed`
- * but i am trying a discipline where contains_not_necessarily_well_typed is not exported
- *)
 abstract let free_mm (#a:Type) (h:heap) (r:ref a{h `contains` r /\ is_mm r})
   :GTot heap
   = { h with memory = (fun r' -> if r' = r.addr then None else h.memory r') }
+
+let modifies (s:set nat) (h0:heap) (h1:heap) =
+  (forall (a:Type) (r:ref a).{:pattern (sel h1 r)}
+                         ((~ (mem (addr_of r) s)) /\ h0 `contains` r) ==> sel h1 r == sel h0 r) /\
+  (forall (a:Type) (r:ref a).{:pattern (contains h1 r)}
+                        h0 `contains` r ==> h1 `contains` r)
 
 (** some lemmas that summarize the behavior **)
 
 (*
  * update of a well-typed reference
  *)
-private let lemma_upd_contains
+private let lemma_upd_contains_test
   (#a:Type) (h0:heap) (r:ref a) (x:a)
   :Lemma (h0 `contains` r ==>
           (let h1 = upd h0 r x in
            (forall (b:Type) (r':ref b). addr_of r' <> addr_of r ==> sel h0 r' == sel h1 r') /\
-	   (forall (b:Type) (r':ref b). h0 `contains` r' ==> h1 `contains` r')             /\
-	   (forall (b:Type) (r':ref b). h0 `contains_not_necessarily_well_typed` r' ==> h1 `contains_not_necessarily_well_typed` r')))
+	   (forall (b:Type) (r':ref b). h0 `contains` r' <==> h1 `contains` r')             /\
+	   (forall (b:Type) (r':ref b). r' `unused_in` h0  <==> r' `unused_in` h1)))
   = ()
 
 (*
  * update of a reference that is mapped but not necessarily well-typed
- * we cannot prove that h0 `contains_a_well_typed` r' ==> h1 `contains_a_well_typed` r'
+ * we cannot prove that h0 `contains` r' ==> h1 `contains` r'
  * because consider that in h0 (r:ref a) contains (| b, y:b |),
  * and that (r':ref b) s.t. r'.addr = r.addr
  * in h0, r' is well-typed, but in h1 it's not
  *)
-private let lemma_upd_contains_not_necessarily_well_typed
+private let lemma_upd_contains_not_necessarily_well_typed_test
   (#a:Type) (h0:heap) (r:ref a) (x:a)
-  :Lemma (h0 `contains_not_necessarily_well_typed` r ==>
+  :Lemma ((~ (r `unused_in` h0)) ==>
           (let h1 = upd h0 r x in
+	   h1 `contains` r /\
            (forall (b:Type) (r':ref b). addr_of r' <> addr_of r ==> sel h0 r' == sel h1 r')           /\
 	   (forall (b:Type) (r':ref b). (r'.addr <> r.addr /\ h0 `contains` r') ==> h1 `contains` r') /\
-	   (forall (b:Type) (r':ref b). h0 `contains_not_necessarily_well_typed` r' ==> h1 `contains_not_necessarily_well_typed` r')))
+	   (forall (b:Type) (r':ref b). r' `unused_in` h0 <==> r' `unused_in` h1)))
   = ()
 
 (*
- * update of an unmapped reference
+ * update of an unused reference
  *)
-private let lemma_upd_unmapped
+private let lemma_upd_unused_test
   (#a:Type) (h0:heap) (r:ref a) (x:a)
-  :Lemma (~ (h0 `contains_not_necessarily_well_typed` r) ==>
+  :Lemma (r `unused_in` h0 ==>
           (let h1 = upd h0 r x in
+	   h1 `contains` r /\
            (forall (b:Type) (r':ref b). addr_of r' <> addr_of r ==> sel h0 r' == sel h1 r') /\
 	   (forall (b:Type) (r':ref b). h0 `contains` r' ==> h1 `contains` r')             /\
-	   (forall (b:Type) (r':ref b). h0 `contains_not_necessarily_well_typed` r' ==> h1 `contains_not_necessarily_well_typed` r')))
+	   (forall (b:Type) (r':ref b). ~ (r' `unused_in` h0) ==> ~ (r' `unused_in` h1))))
   = ()
 
 (*
  * alloc and alloc_mm behaves just like upd of an unmapped reference
  *)
-private let lemma_alloc
-  (#a:Type) (h0:heap) (x:a)
-  :Lemma (let (r, h1) = alloc h0 x in
-          ~ (h0 `contains_not_necessarily_well_typed` r) /\
-	  h1 `contains` r                                /\
-          not (is_mm r)                                                              /\
+private let lemma_alloc_test (#a:Type) (h0:heap) (x:a) (mm:bool)
+  :Lemma (let (r, h1) = alloc h0 x mm in
+          r `unused_in` h0 /\
+	  h1 `contains` r  /\
+          is_mm r = mm     /\
           (forall (b:Type) (r':ref b). addr_of r' <> addr_of r ==> sel h0 r' == sel h1 r') /\
           (forall (b:Type) (r':ref b). h0 `contains` r' ==> h1 `contains` r')             /\
-	  (forall (b:Type) (r':ref b). h0 `contains_not_necessarily_well_typed` r' ==> h1 `contains_not_necessarily_well_typed` r'))
+	  (forall (b:Type) (r':ref b). ~ (r' `unused_in` h0) ==> ~ (r' `unused_in` h1)))
   = ()
 
-private let lemma_alloc_mm
-  (#a:Type) (h0:heap) (x:a)
-  :Lemma (let (r, h1) = alloc_mm h0 x in
-          ~ (h0 `contains_not_necessarily_well_typed` r) /\
-	  h1 `contains` r                                /\
-          is_mm r                                                                    /\
-          (forall (b:Type) (r':ref b). addr_of r' <> addr_of r ==> sel h0 r' == sel h1 r') /\
-	  (forall (b:Type) (r':ref b). h0 `contains` r' ==> h1 `contains` r')             /\
-	  (forall (b:Type) (r':ref b). h0 `contains_not_necessarily_well_typed` r' ==> h1 `contains_not_necessarily_well_typed` r'))
-  = ()
-
-private let lemma_free_mm (#a:Type) (h0:heap) (r:ref a{h0 `contains` r /\ is_mm r})
+private let lemma_free_mm_test (#a:Type) (h0:heap) (r:ref a{h0 `contains` r /\ is_mm r})
   :Lemma (let h1 = free_mm h0 r in
-          (~ (h1 `contains_not_necessarily_well_typed` r)) /\
+          r `unused_in` h1 /\
 	  (forall (b:Type) (r':ref b). addr_of r' <> addr_of r ==>
 	                          ((sel h0 r' == sel h1 r'                 /\
-				   (h0 `contains` r' ==> h1 `contains` r') /\
-				   (h0 `contains_not_necessarily_well_typed` r' ==> h1 `contains_not_necessarily_well_typed` r')))))
+				   (h0 `contains` r' <==> h1 `contains` r') /\
+				   (r' `unused_in` h0 <==> r' `unused_in` h1)))))
+  = ()
+
+private let lemma_upd_modifies_test (#a:Type) (h:heap) (r:ref a{h `contains` r \/ r `unused_in` h}) (x:a)
+  :Lemma (modifies (Set.singleton (addr_of r)) h (upd h r x))
+  = ()
+
+private let lemma_alloc_fresh_test (#a:Type) (h0:heap) (x:a) (mm:bool)
+  :Lemma (let r, h1 = alloc h0 x mm in
+          fresh r h0 h1 /\ modifies empty h0 h1)
+  = ()
+
+private let lemma_modifies_trans_test (h1:heap) (h2:heap) (h3:heap) (s1:set nat) (s2:set nat)
+  :Lemma (requires (modifies s1 h1 h2 /\ modifies s2 h2 h3))
+         (ensures  (modifies (union s1 s2) h1 h3))
   = ()
 
 (** **)
 
-let contains_implies_not_does_not_contain
+let lemma_contains_implies_used
   (#a:Type) (h:heap) (r:ref a)
   :Lemma (requires (h `contains` r))
-         (ensures  (~ (h `does_not_contain` r)))
-	 [SMTPatOr [[SMTPat (h `contains` r)]; [SMTPat (h `does_not_contain` r)]]]
+         (ensures  (~ (r `unused_in` h)))
+	 [SMTPatOr [[SMTPat (h `contains` r)]; [SMTPat (r `unused_in` h)]]]
   = ()
 
-let does_not_contain_addr_of
+let lemma_distinct_addrs
   (#a:Type) (#b:Type) (h:heap) (r1:ref a) (r2:ref b)
-  :Lemma (requires (h `does_not_contain` r1 /\ ~ (h `does_not_contain` r2)))
+  :Lemma (requires (r1 `unused_in` h /\ ~ (r2 `unused_in` h)))
          (ensures  (addr_of r1 <> addr_of r2))
-         [SMTPat (h `does_not_contain` r1); SMTPat (h `does_not_contain` r2)]
+         [SMTPat (r1 `unused_in` h); SMTPat (r2 `unused_in` h)]
   = ()
 
-(*
- * this is as from the previous heap, the pattern also
- *)
-let fresh (s:set nat) (h0:heap) (h1:heap) =
-  forall (a:Type) (r:ref a).{:pattern (h0 `contains_not_necessarily_well_typed` r)}
-                       mem (addr_of r) s ==> (h0 `does_not_contain` r) /\ (h1 `contains` r)
-
-let only x = singleton (addr_of x)
-
-let alloc_lemma (#a:Type) (h0:heap) (x:a)
+let lemma_alloc (#a:Type) (h0:heap) (x:a) (mm:bool)
   :Lemma (requires True)
-         (ensures  (let r, h1 = alloc h0 x in
-                    h1 == upd h0 r x /\ h0 `does_not_contain` r /\ h1 `contains` r /\ not (is_mm r)))
+         (ensures  (let r, h1 = alloc h0 x mm in
+                    h1 == upd h0 r x /\ fresh r h0 h1 /\ is_mm r = mm))
 	 [SMTPat (alloc h0 x)]
   = ()
 
-let alloc_mm_lemma (#a:Type) (h0:heap) (x:a)
-  :Lemma (requires True)
-         (ensures  (let r, h1 = alloc_mm h0 x in
-                    h1 == upd h0 r x /\ h0 `does_not_contain` r /\ h1 `contains` r /\ is_mm r))
-	 [SMTPat (alloc_mm h0 x)]
-  = ()
-
-let free_mm_lemma_sel (#a:Type) (#b:Type) (h0:heap) (r:ref a{h0 `contains` r /\ is_mm r}) (r':ref b)
+let lemma_free_mm_sel (#a:Type) (#b:Type) (h0:heap) (r:ref a{h0 `contains` r /\ is_mm r}) (r':ref b)
   :Lemma (requires True)
          (ensures  (addr_of r' <> addr_of r ==> sel h0 r' == sel (free_mm h0 r) r'))
 	 [SMTPat (sel (free_mm h0 r) r')]
   = ()
 
-let free_mm_does_not_contain_same (#a:Type) (h0:heap) (r:ref a{h0 `contains` r /\ is_mm r})
+let lemma_free_mm_unused (#a:Type) (h0:heap) (r:ref a{h0 `contains` r /\ is_mm r})
   :Lemma (requires True)
-         (ensures  ((free_mm h0 r) `does_not_contain` r))
-	 [SMTPat ((free_mm h0 r) `does_not_contain` r)]
+         (ensures  (r `unused_in` (free_mm h0 r)))
+	 [SMTPat (r `unused_in` (free_mm h0 r))]
   = ()
 
-let free_mm_contains_diff (#a:Type) (#b:Type) (h0:heap) (r:ref a{h0 `contains` r /\ is_mm r}) (r':ref b)
+let lemma_free_mm_contains (#a:Type) (#b:Type) (h0:heap) (r:ref a{h0 `contains` r /\ is_mm r}) (r':ref b)
   :Lemma (requires True)
          (ensures  (let h1 = free_mm h0 r in
 	            (addr_of r' <> addr_of r /\ h0 `contains` r') ==> h1 `contains` r'))
 	 [SMTPat ((free_mm h0 r) `contains` r')]
   = ()
 
-let sel_same_addr (#a:Type) (h:heap) (r1:ref a) (r2:ref a)
+let lemma_sel_same_addr (#a:Type) (h:heap) (r1:ref a) (r2:ref a)
   :Lemma (requires (h `contains` r1 /\ addr_of r1 = addr_of r2))
          (ensures  (h `contains` r2 /\ sel h r1 == sel h r2))
 	 [SMTPat (sel h r1); SMTPat (sel h r2)]
@@ -241,18 +230,8 @@ let sel_upd2 (#a:Type) (#b:Type) (h:heap) (r1:ref a) (r2:ref b) (x:b)
 	 [SMTPat (sel (upd h r2 x) r1)]
   = ()
 
-(*
- * AR: I am pretty sure we can derive it, TODO
- *)
-(* val upd_sel : #a:Type -> h:heap -> r:ref a ->  *)
-(* 	      Lemma (requires (h `contains_a_well_typed` r)) *)
-(* 	            (ensures  (upd h r (sel h r) == h)) *)
-(* 	      [SMTPat (upd h r (sel h r))] *)
-(* let upd_sel #a h r =  *)
-(*   assert (FStar.FunctionalExtensionality.feq (upd h r (sel h r)).memory h.memory) *)
-
 let equal_dom (h1:heap) (h2:heap) :GTot Type0 =
-  forall (a:Type0) (r:ref a). h1 `contains_not_necessarily_well_typed` r <==> h2 `contains_not_necessarily_well_typed` r
+  forall (a:Type0) (r:ref a). r `unused_in` h1 <==> r `unused_in` h2
 
 (* Empty. *)
 let emp :heap = {
@@ -262,19 +241,9 @@ let emp :heap = {
 
 let in_dom_emp (#a:Type) (r:ref a)
   :Lemma (requires True)
-         (ensures  (emp `does_not_contain` r))
-	 [SMTPat (emp `does_not_contain` r)]
+         (ensures  (r `unused_in` emp))
+	 [SMTPat (r `unused_in` emp)]
   = ()
-
-(*
- * see the 3 private lemmas for the behavior of update above
- *)
-(* let upd_contains (#a:Type) (#b:Type) (h:heap) (r:ref a) (x:a) (r':ref b) *)
-(*   :Lemma (requires True) *)
-(*          (ensures  (((upd h r x) `contains` r) /\ *)
-(* 	            (h `contains_not_necessarily_well_typed` r' ==> (upd h r x) `contains_not_necessarily_well_typed` r'))) *)
-(* 	 [SMTPat ((upd h r x) `contains_not_necessarily_well_typed` r')] *)
-(*   = () *)
 
 let upd_contains_a_well_typed (#a:Type) (#b:Type) (h:heap) (r:ref a) (x:a) (r':ref b)
   :Lemma (requires True)
@@ -283,36 +252,12 @@ let upd_contains_a_well_typed (#a:Type) (#b:Type) (h:heap) (r:ref a) (x:a) (r':r
 	            ((h `contains` r' /\  //if h contains_a_well_typed r' and
 
                       ((h `contains` r) \/  //either h contains_a_well_typed r
-		       (h `does_not_contain` r)          \/  //or h does not contain r
-		       (addr_of r <> addr_of r')))             //or r'.addr <> r.addr
+		       (r `unused_in` h) \/  //or h does not contain r
+		       (addr_of r <> addr_of r')))  //or r'.addr <> r.addr
 		     ==> (upd h r x) `contains` r')))  //then updated heap contains_a_well_typed r'
          [SMTPat ((upd h r x) `contains` r')]
   = ()
 
-let modifies (s:set nat) (h0:heap) (h1:heap) =
-  (forall (a:Type) (r:ref a).{:pattern (sel h1 r)}
-                         ((~ (mem (addr_of r) s)) /\ h0 `contains` r) ==> sel h1 r == sel h0 r) /\
-  (forall (a:Type) (r:ref a).{:pattern (contains h1 r)}
-                        h0 `contains` r ==> h1 `contains` r)
-  (* (forall (a:Type) (r:ref a).{:pattern (h1 `contains_not_necessarily_well_typed` r)} *)
-  (*                       h0 `contains_not_necessarily_well_typed` r ==> h1 `contains_not_necessarily_well_typed` r) /\ *)
-  (* (forall (a:Type) (r:ref a).{:pattern (h1 `contains` r)} *)
-  (*                       (~ (mem (addr_of r) s) /\ h0 `contains` r) ==> h1 `contains` r) *)
-
-private let upd_modifies (#a:Type) (h:heap) (r:ref a{h `contains` r \/ h `does_not_contain` r}) (x:a)
-  :Lemma (modifies (Set.singleton (addr_of r)) h (upd h r x))
-  = ()
-
-abstract val lemma_modifies_trans: m1:heap -> m2:heap -> m3:heap
-                       -> s1:set nat -> s2:set nat
-                       -> Lemma (requires (modifies s1 m1 m2 /\ modifies s2 m2 m3))
-                               (ensures (modifies (union s1 s2) m1 m3))
-let lemma_modifies_trans m1 m2 m3 s1 s2 = ()
-
-(*
- * AR: we don't have a public definition of heap equality, which is non-ideal
- * as it requires lemmas like upd_upd_same_ref below
- *)
 abstract let equal (h1:heap) (h2:heap) :Type0 =
   h1.next_addr = h2.next_addr /\
   FStar.FunctionalExtensionality.feq h1.memory h2.memory
